bloom-filter/Proof.BloomFilter.fst
@@ -1,0 +1,260 @@
+module Proof.BloomFilter
+
+module U64 = FStar.UInt64
+module Usize = FStar.UInt32
+module U32 = FStar.UInt32
+module U8 = FStar.UInt8
+module I64 = FStar.Int64
+module Isize = FStar.Int32
+module I32 = FStar.Int32
+
+open Rust
+open Spec.BloomFilter
+open BloomFilter
+
+let modified_only_one_slot
+  (old_bf:bloom_storage_u8)
+  (new_bf:bloom_storage_u8)
+  (idx:valid_index) =
+  forall (idx':valid_index{idx <> idx'}).
+  array_index new_bf.counters idx' = array_index old_bf.counters idx'
+
+let adjust_slot_lemma
+  (bf:bloom_storage_u8)
+  (idx:valid_index)
+  (increment:bool{valid_incr bf idx increment})
+  : Lemma (ensures (
+    let new_bf = adjust_slot bf idx increment in
+    modified_only_one_slot bf new_bf idx /\
+    begin if increment then
+      not (slot_is_empty new_bf idx)
+    else
+      true
+    end
+  )) = ()
+
+let adjust_first_slot_lemma
+  (bf:bloom_storage_u8)
+  (hash:u32)
+  (increment:bool{valid_incr bf (first_slot_index hash) increment})
+  : Lemma (ensures (
+    let new_bf = adjust_first_slot bf hash increment in
+    let idx = first_slot_index hash in
+    modified_only_one_slot bf new_bf idx /\
+    begin if increment then
+      not (slot_is_empty new_bf idx)
+    else
+      true
+    end
+  )) = adjust_slot_lemma bf (first_slot_index hash) increment
+
+let adjust_second_slot_lemma
+  (bf:bloom_storage_u8)
+  (hash:u32)
+  (increment:bool{valid_incr bf (second_slot_index hash) increment})
+  : Lemma (ensures (
+    let new_bf = adjust_second_slot bf hash increment in
+    let idx = second_slot_index hash in
+    modified_only_one_slot bf new_bf idx /\
+    begin if increment then
+      not (slot_is_empty new_bf idx)
+    else
+      true
+    end
+  )) = adjust_slot_lemma bf (second_slot_index hash) increment
+
+
+let modified_hash_slots
+  (old_bf:bloom_storage_u8)
+  (new_bf:bloom_storage_u8)
+  (hash:u32) =
+  let idx1 = first_slot_index hash in
+  let idx2 = second_slot_index hash in
+  forall (idx':valid_index{idx' <> idx1 /\ idx' <> idx2}).
+  array_index new_bf.counters idx' = array_index old_bf.counters idx'
+
+let insert_hash_lemma
+  (bf:bloom_storage_u8)
+  (hash:u32)
+  : Lemma (ensures (
+    let new_bf = insert_hash bf hash in
+    modified_hash_slots bf new_bf hash /\
+    might_contain_hash new_bf hash
+  )) =
+    adjust_first_slot_lemma bf hash true;
+    let bf0 = adjust_first_slot bf hash true in
+    adjust_second_slot_lemma bf0 hash true
+
+let remove_hash_lemma
+  (bf:bloom_storage_u8)
+  (hash:u32)
+  : Lemma (ensures (
+    let new_bf = remove_hash bf hash in
+    modified_hash_slots bf new_bf hash
+  )) =
+  if (first_slot_is_empty bf hash) then () else
+    let bf0 = adjust_first_slot bf hash false in
+    adjust_first_slot_lemma bf hash false;
+    if (second_slot_is_empty bf0 hash) then
+      adjust_first_slot_lemma bf0 hash true
+    else
+      adjust_second_slot_lemma bf0 hash false
+
+let add_only_bloom_filter
+  (bf:bloom_storage_u8)
+  : Tot bool =
+  let elements = bf.ghost_state.elements in
+  all_elements elements (fun e ->
+    might_contain_hash bf (hash e)
+  )
+
+
+let element_invalidation (bf: bloom_storage_u8) =
+  (forall (e:element). (
+    (not (might_contain_hash bf (hash e))) ==>
+      (not (contains bf.ghost_state.elements e))
+  ))
+
+let count_invariant_property (bf:bloom_storage_u8) (e:element) : Tot bool =
+  let hash_e = hash e in
+  let val1 = slot_value bf (first_slot_index hash_e) in
+  let val2 = slot_value bf (second_slot_index hash_e) in
+  begin if U8.v val1 < _MAX_U8 then true else
+    element_count bf.ghost_state.elements e <= U8.v val1
+  end && begin if U8.v val2 < _MAX_U8 then true else
+    element_count bf.ghost_state.elements e <= U8.v val2
+  end
+
+let count_invariant (bf:bloom_storage_u8) : Tot bool =
+  all_elements #element bf.ghost_state.elements (fun e ->
+    count_invariant_property bf e
+  )
+
+let lemma_add_only_bloom_filter
+  (bf: bloom_storage_u8)
+  : Lemma (ensures (
+    add_only_bloom_filter bf <==>
+    (forall (e:element{contains bf.ghost_state.elements e}).
+      might_contain_hash bf (hash e))
+  )) =
+    all_elements_lemma
+      #element
+      bf.ghost_state.elements
+      (fun e -> might_contain_hash bf (hash e))
+
+let lemma_count_invariant (bf:bloom_storage_u8)
+  : Lemma (ensures (count_invariant bf <==>
+    (forall (e:element{contains bf.ghost_state.elements e}).
+    count_invariant_property bf e)
+  )) =
+  all_elements_lemma #element bf.ghost_state.elements
+   (fun e -> count_invariant_property bf e)
+
+type valid_bloom_storage_u8 = bf:bloom_storage_u8{element_invalidation bf /\ count_invariant bf}
+
+type add_only_bloom_storage_u8 = bf:valid_bloom_storage_u8{add_only_bloom_filter bf}
+
+let lemma_insert_hash_prelim
+  (bf: bloom_storage_u8)
+  (idx: valid_index)
+  : Lemma (requires (U8.v (slot_value bf idx) < _MAX_U8))
+    (ensures (U8.v (slot_value (adjust_slot bf idx true) idx) = U8.v (slot_value bf idx) + 1)) =
+    ()
+
+let lemma_insert_hash1
+  (bf: bloom_storage_u8)
+  (hash:u32)
+  : Lemma (requires (
+      U8.v (slot_value bf (first_slot_index hash)) < _MAX_U8)
+    )
+    (ensures (
+      U8.v (slot_value (insert_hash bf hash) (first_slot_index hash)) >
+	U8.v (slot_value bf (first_slot_index hash))
+    )) =
+    lemma_insert_hash_prelim bf (first_slot_index hash)
+
+let lemma_insert_hash2
+  (bf: bloom_storage_u8)
+  (hash:u32)
+  : Lemma (requires (
+      U8.v (slot_value bf (second_slot_index hash)) < _MAX_U8)
+    )
+    (ensures (
+      U8.v (slot_value (insert_hash bf hash) (second_slot_index hash)) >
+	U8.v (slot_value bf (second_slot_index hash))
+    )) =
+    let idx = second_slot_index hash in
+    if idx = first_slot_index hash then
+      lemma_insert_hash1 bf hash
+    else begin
+      let new_bf0 = adjust_first_slot bf hash true in
+      lemma_insert_hash_prelim new_bf0 (second_slot_index hash)
+    end
+
+(*
+ (* *) lemma_count_invariant bf;
+  (* *) lemma_count_invariant new_bf;
+  let inner_lemma
+    (e':element{contains new_bf.ghost_state.elements e'})
+    : Lemma (ensures (count_invariant_property new_bf e'))
+  =
+    let hash_e' = hash e' in
+    let idx1_e = first_slot_index (hash e) in
+    let idx1_e' = first_slot_index (hash e') in
+    let idx2_e = second_slot_index (hash e) in
+    let idx2_e' = second_slot_index (hash e') in
+    let new_val1 = slot_value new_bf idx1_e' in
+    let new_val2 = slot_value new_bf idx2_e'  in
+    let old_val1 = slot_value bf idx1_e' in
+    let old_val2 = slot_value bf idx2_e' in
+    if U8.v old_val1 = _MAX_U8 then () else
+    assert(U8.v old_val1 < _MAX_U8);
+    begin if idx1_e' = idx1_e || idx1_e' = idx2_e then begin
+      Classical.or_elim
+        #(idx1_e' = idx1_e)
+        #(idx1_e' = idx2_e)
+        #(fun _ -> U8.(old_val1 <=^ new_val1))
+        (fun _ ->
+	  //admit();
+	  lemma_insert_hash_prelim bf idx1_e;
+	  admit()
+	)
+        (fun _ ->
+	  admit();
+	  lemma_insert_hash_prelim bf idx2_e;
+	  admit()
+	);
+       admit()
+    end else
+      admit()
+    end;
+    admit()
+
+
+(*
+    begin if U8.v val1 < _MAX_U8 then () else
+     begin if idx1_e' = idx1_e || idx1_e' = idx2_e then begin
+       if U8.v (slot_value bf idx1_e') < _MAX_U8 then
+         admit()
+       else
+         assert(U8.v (slot_value new_bf idx1_e') = _MAX_U8);
+	 assert(U8.v val1 = _MAX_U8 /\ U8.v val1 < _MAX_U8);
+	 lemma_contradiction new_bf e' val1;
+	 admit()
+       end else begin
+         assert(slot_value bf idx1_e' = slot_value new_bf idx1_e');
+	 assert(count_invariant_property bf e');
+	 assert(element_count bf.ghost_state.elements e' <= U8.v val1)
+       end
+     end
+     //assume(element_count new_bf.ghost_state.elements e' <= U8.v val1)
+    end;
+    begin if U8.v val2 < _MAX_U8 then () else
+      assume(element_count new_bf.ghost_state.elements e' <= U8.v val2)
+    end
+ *)
+  in
+  (* *) Classical.forall_intro inner_lemma;
+  (* *) lemma_add_only_bloom_filter bf;
+  (* *) lemma_add_only_bloom_filter new_bf;
+  *)
